done

Lab3Dafny.dfy
@@ -1,5 +1,10 @@
 // class CircularMemory
 // This class implements a cicular buffer with with 2 int typed pointers
+
+/*
+Authors: Adam Williams, Jonathan Naumanen, Alexander Stenström
+Group: 15
+*/
 class CircularMemory
 {
   var cells : array<int>;
@@ -7,96 +12,108 @@ class CircularMemory
   var write_position : int;
   var isFlipped : bool;
 
-
-  constructor Init(cap : int) 
-    requires cap > 0;
-    ensures cells.Length == cap;
-    ensures read_position == 0;
-    ensures write_position == 0;
-    ensures isFlipped == false;
+  constructor Init(cap : int)
+    requires cap > 0
+    ensures cap == cells.Length
+    ensures read_position == 0
+    ensures write_position == 0
+    ensures isFlipped == false
   {
     cells := new int[cap];
-    read_position := 0;
-    write_position := 0;
+    read_position, write_position := 0, 0;
     isFlipped := false;
-    // missing some pre-condition checks
-  }
-  predicate Valid()
-    reads this
-  {
-    cells.Length > 0 &&
-    read_position >= 0 && read_position < cells.Length &&
-    write_position >= 0 && write_position < cells.Length &&
-    (isFlipped ==> read_position <= write_position) &&
-    (!isFlipped ==> read_position > write_position)
   }
 
-    
+  predicate Valid() 
+    reads this
+  {
+    // array can't be less than 1
+    0 < cells.Length &&
+    //write position needs to be inside index boundaries
+    0 <= write_position < cells.Length && 
+    //same with read position
+    0 <= read_position < cells.Length && 
+    //if the array is flipped, the write position needs to be greater than the read position
+    (isFlipped ==> write_position <= read_position) && 
+    //if the array is not flipped, the write position needs to be less than the read position
+    (!isFlipped ==> write_position >= read_position)
+  }
+
   predicate isEmpty()
     reads this
-    requires Valid();
-    ensures isEmpty() <==> (read_position == write_position && !isFlipped);
   {
     read_position == write_position && !isFlipped
   }
 
   predicate isFull()
     reads this
-    requires Valid();
-    ensures isFull() <==> (read_position == write_position && isFlipped);
   {
     read_position == write_position && isFlipped
   }
 
-
   method Read() returns (isSuccess : bool, content : int)
     modifies this
-    requires Valid();
-    requires !isEmpty();
-    ensures Valid();
-    ensures isSuccess ==> content == old(cells[read_position]);
-    ensures !isSuccess ==> content == 0;
-    ensures cells.Length == old(cells.Length);
+    requires Valid()
+    ensures Valid()
+    ensures  isSuccess ==> content == old(cells[(read_position)])
+    ensures !isSuccess ==> content == 0
+    ensures !isSuccess ==> read_position == old(read_position)
+    ensures cells.Length == old(cells.Length)
   {
-    if(isFlipped) // returns current and advances read position 
+    if(isFlipped) //om flipped write kan inte gå förbi read om !flipped read kan inte gå förbi write
     {
-      isSuccess := false;
-      content := 0;   
-    }
-    else {
       isSuccess := true;
       content := cells[read_position];
       read_position := read_position + 1;
-      if(read_position == cells.Length) {
-        isFlipped := true;
+      if(read_position == cells.Length){
+        isFlipped := false;
         read_position := 0;
+      }
+    }
+    else // not flipped
+    {
+      if(read_position == write_position){
+        isSuccess := false;
+        content := 0;
+      } 
+      else {
+      isSuccess := true;
+      content := cells[read_position];
+      read_position := read_position + 1;
       }
     }
   }
 
   method Write(input : int) returns (isSuccess : bool)
-    modifies this
-    modifies cells[write_position]
-    requires Valid();
-    requires !isFull();
-    ensures Valid();
-    ensures isSuccess ==> input == old(cells[write_position]);
-    ensures !isSuccess ==> cells[write_position] == old(cells[write_position]);
-    ensures cells.Length == old(cells.Length);
+    modifies cells, `write_position, `isFlipped
+    requires Valid()
+    ensures Valid()
+    ensures  isSuccess ==> cells[old(write_position)] == input
+    ensures !isSuccess ==> cells[(write_position)] == old(cells[(write_position)])
+    ensures !isSuccess ==> write_position == old(write_position)
+    ensures cells.Length == old(cells.Length)
   {
-    if(isFlipped) // writes input and advances write position
+    if(!isFlipped)
     {
       isSuccess := true;
-      cells[write_position] := input;
-      write_position := write_position + 1;
-      if(write_position == cells.Length) {
-        isFlipped := false;
+      cells[write_position] := input; 
+      write_position := (write_position + 1);
+      if(write_position == cells.Length){
         write_position := 0;
+        isFlipped := true;
       }
     }
-    else {
-      isSuccess := false;
+    else // flipped
+    {
+      if(write_position == read_position){
+        isSuccess := false;
+      } 
+      else {
+      isSuccess := true;
+      cells[write_position] := input; 
+      write_position := (write_position + 1);
+      }
     }
-  }
 
+  }
 }
